examples/low-level/crypto/Crypto.AEAD.Wrappers.Encoding.fst
@@ -23,7 +23,9 @@ module CMA = Crypto.Symmetric.UF1CMA
 
 module Cipher   = Crypto.Symmetric.Cipher
 module PRF      = Crypto.Symmetric.PRF
+
 open Crypto.AEAD.Encoding
+open Crypto.AEAD.Invariant
 
 ////////////////////////////////////////////////////////////////////////////////
 //AEAD.Encoding.accumulate wrapper
@@ -51,14 +53,14 @@ let accumulate_ensures (#i: MAC.id) (st: CMA.state i)
 		       (#aadlen:aadlen_32) (aad:lbuffer (v aadlen))
 		       (#txtlen:txtlen_32) (cipher:lbuffer (v txtlen))
 		       (h0:mem) (a:CMA.accBuffer i) (h1:mem) =
-  let open HS in		       
-  let open CMA in 		       
+  let open HS in
+  let open CMA in
   accumulate_liveness st aad cipher h1 /\
-  fresh_sref h0 h1 (Buffer.content (MAC.as_buffer a.a)) /\
+  fresh_sref h0 h1 (Buffer.content (MAC.as_buffer (abuf a))) /\
   CMA.acc_inv st a h1 /\
   (mac_log ==> 
-    fresh_sref h0 h1 (alog a) /\
-    HS.sel h1 (alog a) == encode_both (fst i) aadlen (Buffer.as_seq h1 aad) txtlen (Buffer.as_seq h1 cipher))
+    fresh_sref h0 h1 (CMA.alog a) /\
+    HS.sel h1 (CMA.alog a) == encode_both (fst i) aadlen (Buffer.as_seq h1 aad) txtlen (Buffer.as_seq h1 cipher))
 
 val frame_accumulate_ensures: #i: MAC.id -> st: CMA.state i -> #aadlen:aadlen_32 -> aad:lbuffer (v aadlen) ->
 	       #txtlen:txtlen_32 -> cipher:lbuffer (v txtlen) -> 
@@ -70,9 +72,9 @@ val frame_accumulate_ensures: #i: MAC.id -> st: CMA.state i -> #aadlen:aadlen_32
 let frame_accumulate_ensures #i st #aalen aad #txtlent cipher h0 a h1 h2 = 
   FStar.Buffer.lemma_reveal_modifies_0 h1 h2;
   assert (HS.(h1.tip == h2.tip));
-  assert (h1 `HS.contains` (Buffer.content (MAC.as_buffer CMA.(a.a))));
-  assert (h2 `HS.contains` (Buffer.content (MAC.as_buffer CMA.(a.a))));  
-  assert (fresh_sref h0 h2 (Buffer.content (MAC.as_buffer CMA.(a.a))));
+  assert (h1 `HS.contains` (Buffer.content (MAC.as_buffer (CMA.abuf a))));
+  assert (h2 `HS.contains` (Buffer.content (MAC.as_buffer (CMA.abuf a))));
+  assert (fresh_sref h0 h2 (Buffer.content (MAC.as_buffer (CMA.abuf a))));
   if mac_log 
   then (assert (h1  `HS.contains` CMA.alog a);
         assert (HS.sel h2 (CMA.alog a) == HS.sel h1 (CMA.alog a));
@@ -84,20 +86,45 @@ let frame_accumulate_ensures #i st #aalen aad #txtlent cipher h0 a h1 h2 =
         MAC.frame_sel_elem h1 h2 (CMA.(abuf a)))
   else ()
 
-let accumulate (#i: MAC.id) (st: CMA.state i) (#aadlen:aadlen_32) (aad:lbuffer (v aadlen))
-	       (#txtlen:txtlen_32) (cipher:lbuffer (v txtlen))
-   : StackInline (CMA.accBuffer i)
+unfold let accumulate_ensures' (#i: MAC.id) (st: CMA.state i) 
+		       (#aadlen:aadlen_32) (aad:lbuffer (v aadlen))
+		       (#txtlen:txtlen_32) (cipher:lbuffer (v txtlen))
+		       (h0:mem) (a:CMA.accBuffer i) (h1:mem) =
+  let open HS in
+  let open CMA in
+  accumulate_liveness st aad cipher h1 /\
+  fresh_sref h0 h1 (Buffer.content (MAC.as_buffer (abuf a))) /\
+  CMA.acc_inv st a h1 /\
+  (mac_log ==> 
+    fresh_sref h0 h1 (CMA.alog a) /\
+    HS.sel h1 (CMA.alog a) == encode_both (fst i) aadlen (Buffer.as_seq h1 aad) txtlen (Buffer.as_seq h1 cipher))
+
+let accumulate (#i: id) (#rw:rw) (#n:Cipher.iv (Cipher.algi i)) (aead_st:aead_state i rw)
+	       (ak: CMA.state (i, n)) (#aadlen:aadlen_32) (aad:lbuffer (v aadlen))
+	       (#txtlen:txtlen_32) (plain:plainBuffer i (v txtlen)) (cipher_tagged:lbuffer (v txtlen + v MAC.taglen))
+   : StackInline (CMA.accBuffer (i, n))
       (requires (fun h0 -> 
-	  accumulate_liveness st aad cipher h0))
+	  enc_dec_liveness aead_st aad plain cipher_tagged h0 /\ 
+	  MAC.norm h0 CMA.(ak.r) /\
+	  (safeId i ==> is_mac_for_iv aead_st ak h0) /\
+	  inv aead_st h0))
       (ensures (fun h0 a h1 ->  
-      	  accumulate_liveness st aad cipher h0 /\
+	  let cipher : lbuffer (v txtlen) = Buffer.sub cipher_tagged 0ul txtlen in
+      	  enc_dec_liveness aead_st aad plain cipher_tagged h1 /\ 
+  	  MAC.norm h1 CMA.(ak.r) /\
+  	  (safeId i ==> is_mac_for_iv aead_st ak h1) /\
           accumulate_modifies_nothing h0 h1 /\
-	  accumulate_ensures st aad cipher h0 a h1))
+	  accumulate_ensures ak aad cipher h0 a h1 /\
+	  inv aead_st h1))
   = let h0 = get () in
-    let acc = accumulate #i st aadlen aad txtlen cipher in
+    let cipher : lbuffer (v txtlen) = Buffer.sub cipher_tagged 0ul txtlen in
+    let acc = accumulate #(i, n) ak aadlen aad txtlen cipher in
     let h1 = get () in
-    assert (Buffer.disjoint_2 (MAC.as_buffer (CMA.(acc.a))) (CMA.(st.s)) cipher);
+    assert (Buffer.disjoint_2 (MAC.as_buffer (CMA.abuf acc)) (CMA.(ak.s)) cipher);
     assume (mac_log ==> fresh_sref h0 h1 (CMA.alog acc)); //NS: this goes away when Encoding.accumulate is restored
-    assume (fresh_sref h0 h1 (Buffer.content (MAC.as_buffer CMA.(acc.a))));
+    assume (fresh_sref h0 h1 (Buffer.content (MAC.as_buffer (CMA.abuf acc))));
     FStar.Buffer.lemma_reveal_modifies_0 h0 h1;
+    frame_inv_modifies_tip aead_st h0 h1;
+    assert (accumulate_ensures' ak aad cipher h0 acc h1);
+    assume (accumulate_ensures ak aad cipher h0 acc h1); //NS:weirdness, can prove something equivalent up to unfolding
     acc
